MemOpsFuncs.v
@@ -45,13 +45,13 @@ Section memOpsFuncs.
     := unpack DataMask
          ($(Nat.pow 2 (Nat.pow 2 size) - 1)).
 
-  Definition getMaskExpr ty
-    (sz : TlSize @# ty)
+  Definition getMaskExpr ty n
+    (sz : Bit n @# ty)
     :  Bit (size DataMask) @# ty
     := ($1 << (($1 : Bit (S (Nat.log2_up Rlen_over_8)) @# ty) << sz)) - $1.
 
-  Definition getMaskShiftAmt ty
-    (sz : TlSize @# ty)
+  Definition getMaskShiftAmt ty n
+    (sz : Bit n @# ty)
     (address : PAddr @# ty)
     :  Bit 3 @# ty
     := ((ZeroExtendTruncLsb 3 address) >> sz) << sz.
